Add more stuff to combinators (naive: const_recv)

dimsum/iris/combinators.v
@@ -627,13 +627,18 @@ Section link.
     iApply ("Hsim" with "[$] [$]").
   Qed.
 
-
-  Lemma sim_tgt_link_left_recv R m1 m2 s σ1 σ2 Π e :
-    (σ1 ≈{m1}≈>ₜ λ κ σ1',
+  Definition link_tgt_left_recvP R {m1 m2 : mod_trans (io_event EV)}
+    (Π : option (io_event EV) → link_case EV * S * m_state m1 * m_state m2 → iProp Σ)
+    (s : S) (σ2 : m_state m2) e : option (io_event EV) → m_state m1 → iProp Σ :=
+    λ κ σ1',
       match κ with
       | None => Π None (MLFRecv SPLeft e, s, σ1', σ2)
-      | Some e' => ⌜e' = (Incoming, e)⌝ -∗ (MLFRun (Some SPLeft), s, σ1', σ2) ≈{link_trans R m1 m2}≈>ₜ Π
-      end%I) -∗
+      | Some e' => ⌜e' = (Incoming, e)⌝ -∗
+                   (MLFRun (Some SPLeft), s, σ1', σ2) ≈{link_trans R m1 m2}≈>ₜ Π
+      end%I.
+
+  Lemma sim_tgt_link_left_recv R m1 m2 s σ1 σ2 Π e :
+    σ1 ≈{m1}≈>ₜ link_tgt_left_recvP R Π s σ2 e -∗
     (MLFRecv SPLeft e, s, σ1, σ2) ≈{link_trans R m1 m2}≈>ₜ Π.
   Proof.
     iIntros "Hsim".
@@ -646,6 +651,27 @@ Section link.
     iIntros ([[[??]?]?]?). simplify_eq/=. destruct κ; destruct!/=.
     - inv_all @link_filter. iRight. iSplit!. by iApply "Hsim".
     - by iLeft.
+  Qed.
+
+  Definition link_tgt_left_recv_constP R {m1 m2 : mod_trans (io_event EV)}
+    (Π : option (io_event EV) → link_case EV * S * m_state m1 * m_state m2 → iProp Σ)
+    (γ_s γ_σ2 γ_e : gname) : option (io_event EV) → m_state m1 → iProp Σ :=
+    λ κ σ1', (∀ s σ2 e, γ_s ⤳ s -∗ γ_σ2 ⤳ σ2 -∗ γ_e ⤳ e -∗ link_tgt_left_recvP R Π s σ2 e κ σ1')%I.
+
+  Lemma sim_tgt_link_left_recv_const R m1 m2 s σ1 σ2 e γ_s γ_σ2 γ_e Π :
+    γ_s ⤳@{S} - -∗
+    γ_σ2 ⤳@{m_state m2} - -∗
+    γ_e ⤳@{EV}- -∗
+    (γ_s ⤳ s -∗ γ_σ2 ⤳ σ2 -∗ γ_e ⤳ e -∗ σ1 ≈{m1}≈>ₜ link_tgt_left_recv_constP R Π γ_s γ_σ2 γ_e) -∗
+    (MLFRecv SPLeft e, s, σ1, σ2) ≈{link_trans R m1 m2}≈>ₜ Π.
+  Proof.
+    iIntros "Hγ_s Hγ_σ2 Hγ_e Hsim".
+    iMod (mstate_var_split γ_s with "Hγ_s") as "[??]".
+    iMod (mstate_var_split γ_σ2 with "Hγ_σ2") as "[??]".
+    iMod (mstate_var_split γ_e with "Hγ_e") as "[??]".
+    iApply sim_tgt_link_left_recv. iSpecialize ("Hsim" with "[$] [$] [$]").
+    iApply (sim_gen_wand with "Hsim"). iIntros (??) "Hsim".
+    iApply ("Hsim" with "[$] [$] [$]").
   Qed.
 
   Definition link_tgt_rightP R {m1 m2 : mod_trans (io_event EV)}
@@ -684,16 +710,22 @@ Section link.
     - iIntros ([[[??]?]?] ?). simplify_eq/=. by iLeft.
   Qed.
 
-  Lemma sim_tgt_link_right_recv R m1 m2 s σ1 σ2 Π e :
-    (σ2 ≈{m2}≈>ₜ λ κ σ2',
+  Definition link_tgt_right_recvP R {m1 m2 : mod_trans (io_event EV)}
+    (Π : option (io_event EV) → link_case EV * S * m_state m1 * m_state m2 → iProp Σ)
+    (s : S) (σ1 : m_state m1) e : option (io_event EV) → m_state m2 → iProp Σ :=
+    λ κ σ2',
       match κ with
       | None => Π None (MLFRecv SPRight e, s, σ1, σ2')
-      | Some e' => ⌜e' = (Incoming, e)⌝ -∗ (MLFRun (Some SPRight), s, σ1, σ2') ≈{link_trans R m1 m2}≈>ₜ Π
-      end%I) -∗
+      | Some e' => ⌜e' = (Incoming, e)⌝ -∗
+                   (MLFRun (Some SPRight), s, σ1, σ2') ≈{link_trans R m1 m2}≈>ₜ Π
+      end%I.
+
+  Lemma sim_tgt_link_right_recv R m1 m2 s σ1 σ2 Π e :
+    σ2 ≈{m2}≈>ₜ link_tgt_right_recvP R Π s σ1 e -∗
     (MLFRecv SPRight e, s, σ1, σ2) ≈{link_trans R m1 m2}≈>ₜ Π.
   Proof.
     iIntros "Hsim".
-    iApply sim_gen_bind.
+    iApply (sim_gen_bind with "[-]").
     iApply sim_tgt_state_transform; [done|] => /=.
     iApply (sim_tgt_map with "[-]").
     iApply sim_tgt_seq_product_right.
